src/lib/DenseOrder.v
@@ -2,19 +2,19 @@ Require Import Orders.
 Require Import OrdersFacts.
 Require Import RelationClasses.
 Require Import PArith.
+Require Import FMapPositive.
 
 Require Import sflib.
 Require Import paco.
 
+Require Import Axioms.
 Require Import Basic.
 Require Import DataStructure.
 Require Import UsualFMapPositive.
 
 Module Type IsDense (Import T:EqLtLe).
-  Parameter elt: t.
-
-  Parameter decr: t -> t.
-  Axiom decr_spec: forall x, lt (decr x) x.
+  Parameter bot: t.
+  Axiom bot_spec: forall x, le bot x.
 
   Parameter incr: t -> t.
   Axiom incr_spec: forall x, lt x (incr x).
@@ -29,7 +29,7 @@ End IsDense.
 
 Module Type DenseOrderType := UsualOrderedTypeFull <+ IsDense <+ HasCaseJoin.
 
-Module DenseOrder <: DenseOrderType.
+Module DOAux.
   Definition t := positive.
   Definition elt: t := xH.
 
@@ -83,46 +83,46 @@ Module DenseOrder <: DenseOrderType.
     | xI ltl, xI rtl =>
       compare ltl rtl
     end.
-   Lemma compare_spec :
-     forall x y : t,
-       CompareSpec (x = y) (lt x y) (lt y x) (compare x y).
-   Proof.
-     induction x; i; destruct y;
-       try (destruct a);
-       try (destruct b);
-       repeat (try econs; s).
-     - destruct (IHx y); subst; repeat econs; auto.
-     - destruct (IHx y); subst; repeat econs; auto.
-   Qed.
+  Lemma compare_spec :
+    forall x y : t,
+      CompareSpec (x = y) (lt x y) (lt y x) (compare x y).
+  Proof.
+    induction x; i; destruct y;
+      try (destruct a);
+      try (destruct b);
+      repeat (try econs; s).
+    - destruct (IHx y); subst; repeat econs; auto.
+    - destruct (IHx y); subst; repeat econs; auto.
+  Qed.
 
-   Lemma eq_dec: forall x y : t, {x = y} + {x <> y}.
-   Proof.
-     apply Pos.eq_dec.
-   Defined.
-   Global Opaque eq_dec.
+  Lemma eq_dec: forall x y : t, {x = y} + {x <> y}.
+  Proof.
+    apply Pos.eq_dec.
+  Defined.
+  Global Opaque eq_dec.
 
-   Definition le := lt \2/ eq.
-   Lemma le_lteq : forall x y : t, le x y <-> lt x y \/ x = y.
-   Proof. auto. Qed.
-   Global Opaque le.
+  Definition le := lt \2/ eq.
+  Lemma le_lteq : forall x y : t, le x y <-> lt x y \/ x = y.
+  Proof. auto. Qed.
+  Global Opaque le.
 
-   Fixpoint decr (x:t) :=
-     match x with
-     | xH => xO xH
-     | xO x => xO (decr x)
-     | xI x => xI (decr x)
-     end.
+  Fixpoint decr (x:t) :=
+    match x with
+    | xH => xO xH
+    | xO x => xO (decr x)
+    | xI x => xI (decr x)
+    end.
 
   Lemma decr_spec: forall x, lt (decr x) x.
     induction x; ss; econs; eauto.
   Qed.
 
-   Fixpoint incr (x:t) :=
-     match x with
-     | xH => xI xH
-     | xO x => xO (incr x)
-     | xI x => xI (incr x)
-     end.
+  Fixpoint incr (x:t) :=
+    match x with
+    | xH => xI xH
+    | xO x => xO (incr x)
+    | xI x => xI (incr x)
+    end.
 
   Lemma incr_spec: forall x, lt x (incr x).
     induction x; ss; econs; eauto.
@@ -130,10 +130,10 @@ Module DenseOrder <: DenseOrderType.
 
   Fixpoint middle (lhs rhs:t): t :=
     match lhs, rhs with
-    | xH, rhs => decr rhs
     | lhs, xH => incr lhs
+    | xH, rhs => decr rhs
     | xO ltl, xO rtl => xO (middle ltl rtl)
-    | xO ltl, xI rtl => xO (incr ltl)
+    | xO ltl, xI rtl => xI (decr rtl)
     | xI ltl, xO rtl => xI (middle ltl rtl)
     | xI ltl, xI rtl => xI (middle ltl rtl)
     end.
@@ -314,6 +314,311 @@ Module DenseOrder <: DenseOrderType.
     - left. econs. auto.
     - inv H. right. refl.
   Qed.
+End DOAux.
+
+Global Program Instance DOAux_le_PreOrder: PreOrder DOAux.le.
+Next Obligation.
+  ii. apply DOAux.le_lteq. right. auto.
+Qed.
+Next Obligation.
+  ii. apply DOAux.le_lteq.
+  apply DOAux.le_lteq in H.
+  apply DOAux.le_lteq in H0.
+  des; subst; auto.
+  left. rewrite H. auto.
+Qed.
+
+Module DenseOrder.
+  Definition t := positive.
+
+  Definition eq := @eq t.
+  Global Program Instance eq_equiv : Equivalence eq.
+
+  Inductive lt_: forall (lhs rhs:t), Prop :=
+  | lt_xH_xO lhs:
+      lt_ xH (xO lhs)
+  | lt_xH_xI lhs:
+      lt_ xH (xI lhs)
+  | lt_xO_xI lhs rhs:
+      lt_ (xO lhs) (xI rhs)
+  | lt_xO
+      lhs rhs
+      (LT: DOAux.lt lhs rhs):
+      lt_ (xO lhs) (xO rhs)
+  | lt_xI
+      lhs rhs
+      (LT: DOAux.lt lhs rhs):
+      lt_ (xI lhs) (xI rhs)
+  .
+  Definition lt := lt_.
+  Global Program Instance lt_strorder: StrictOrder lt.
+  Next Obligation.
+    ii. inv H.
+    - eapply DOAux.lt_strorder. eauto.
+    - eapply DOAux.lt_strorder. eauto.
+  Qed.
+  Next Obligation.
+    ii. inv H; inv H0; econs.
+    - etrans; eauto.
+    - etrans; eauto.
+  Qed.
+  Global Program Instance lt_compat: Proper (eq ==> eq ==> iff) lt.
+  Next Obligation.
+    ii. unfold eq in *. subst. auto.
+  Qed.
+  Fixpoint compare (lhs rhs:t): comparison :=
+    match lhs, rhs with
+    | xH, xH =>
+      Eq
+    | xH, xO _
+    | xH, xI _
+    | xO _, xI _ =>
+      Lt
+    | xO _, xH
+    | xI _, xO _
+    | xI _, xH =>
+      Gt
+    | xO ltl, xO rtl
+    | xI ltl, xI rtl =>
+      DOAux.compare ltl rtl
+    end.
+  Lemma compare_spec :
+    forall x y : t,
+      CompareSpec (x = y) (lt x y) (lt y x) (compare x y).
+  Proof.
+    i. destruct x, y; s; try by repeat econs.
+    - generalize (DOAux.compare_spec x y).
+      destruct (DOAux.compare x y); i; inv H.
+      + econs 1. auto.
+      + econs 2. econs. auto.
+      + econs 3. econs. auto.
+    - generalize (DOAux.compare_spec x y).
+      destruct (DOAux.compare x y); i; inv H.
+      + econs 1. auto.
+      + econs 2. econs. auto.
+      + econs 3. econs. auto.
+  Qed.
+
+  Lemma eq_dec: forall x y : t, {x = y} + {x <> y}.
+  Proof.
+    apply Pos.eq_dec.
+  Defined.
+  Global Opaque eq_dec.
+
+  Definition le := lt \2/ eq.
+  Lemma le_lteq : forall x y : t, le x y <-> lt x y \/ x = y.
+  Proof. auto. Qed.
+  Global Opaque le.
+
+  Definition bot: t := xH.
+
+  Lemma bot_spec: forall x, le bot x.
+  Proof.
+    i. destruct x.
+    - left. econs.
+    - left. econs.
+    - right. refl.
+  Qed.
+
+  Fixpoint incr (x:t) :=
+    match x with
+    | xH => xI xH
+    | xO x => xO (DOAux.incr x)
+    | xI x => xI (DOAux.incr x)
+    end.
+
+  Lemma incr_spec: forall x, lt x (incr x).
+    i. destruct x; econs.
+    - apply DOAux.incr_spec.
+    - apply DOAux.incr_spec.
+  Qed.
+
+  Fixpoint middle (lhs rhs:t): t :=
+    match lhs, rhs with
+    | _, xH => lhs
+    | xH, xO rtl => xO (DOAux.decr rtl)
+    | xH, xI _ => xO xH
+    | xO ltl, xO rtl => xO (DOAux.middle ltl rtl)
+    | xO ltl, xI rtl => xI (DOAux.decr rtl)
+    | xI ltl, xO rtl => xI (DOAux.middle ltl rtl)
+    | xI ltl, xI rtl => xI (DOAux.middle ltl rtl)
+    end.
+
+  Lemma middle_spec:
+    forall (lhs rhs:t)
+      (LT: lt lhs rhs),
+      lt lhs (middle lhs rhs) /\
+      lt (middle lhs rhs) rhs.
+  Proof.
+    i. inv LT; s; splits; econs;
+         (try apply DOAux.decr_spec);
+         (try apply DOAux.middle_spec; auto).
+  Qed.
+
+  Lemma le_lt_dec (lhs rhs:t): {le lhs rhs} + {lt rhs lhs}.
+  Proof.
+    generalize (compare_spec lhs rhs).
+    destruct (compare lhs rhs).
+    - left. inv H. right. ss.
+    - left. inv H. apply le_lteq. auto.
+    - right. inv H. auto.
+  Defined.
+
+  Definition join (lhs rhs:t): t :=
+    if le_lt_dec lhs rhs
+    then rhs
+    else lhs.
+
+  Lemma join_comm lhs rhs: join lhs rhs = join rhs lhs.
+  Proof.
+    unfold join.
+    destruct (le_lt_dec lhs rhs), (le_lt_dec rhs lhs); auto.
+    - apply le_lteq in l. apply le_lteq in l0.
+      des; auto. rewrite l in l0. apply lt_strorder in l0. done.
+    - rewrite l in l0. apply lt_strorder in l0. done.
+  Qed.
+
+  Lemma join_assoc a b c: join (join a b) c = join a (join b c).
+  Proof.
+    unfold join.
+    repeat
+      (try match goal with
+           | [H: le _ _ |- _] =>
+             apply le_lteq in H
+           | [|- context[le_lt_dec ?a ?b]] =>
+             destruct (le_lt_dec a b)
+           | [H: context[le_lt_dec ?a ?b] |- _] =>
+             destruct (le_lt_dec a b)
+           | [H1: lt ?a ?b, H2: lt ?b ?a |- _] =>
+             rewrite H2 in H1; apply lt_strorder in H1; inv H1
+           end; unfold eq in *; try subst; des; ss).
+    - rewrite l in l2. rewrite l0 in l2.
+      apply lt_strorder in l2. inv l2.
+    - rewrite l in l2. rewrite l1 in l2.
+      apply lt_strorder in l2. inv l2.
+  Qed.
+
+  Lemma join_l lhs rhs:
+    le lhs (join lhs rhs).
+  Proof.
+    unfold join. destruct (le_lt_dec lhs rhs); auto.
+    apply le_lteq. auto.
+  Qed.
+
+  Lemma join_r lhs rhs:
+    le rhs (join lhs rhs).
+  Proof.
+    rewrite join_comm. apply join_l.
+  Qed.
+
+  Lemma join_spec lhs rhs o
+        (LHS: le lhs o)
+        (RHS: le rhs o):
+    le (join lhs rhs) o.
+  Proof.
+    unfold join. destruct (le_lt_dec lhs rhs); auto.
+  Qed.
+
+  Lemma join_cases lhs rhs:
+    join lhs rhs = lhs \/ join lhs rhs = rhs.
+  Proof.
+    unfold join. destruct (le_lt_dec lhs rhs); auto.
+  Qed.
+
+  Definition meet (lhs rhs:t): t :=
+    if le_lt_dec lhs rhs
+    then lhs
+    else rhs.
+
+  Lemma meet_comm lhs rhs: meet lhs rhs = meet rhs lhs.
+  Proof.
+    unfold meet.
+    destruct (le_lt_dec lhs rhs), (le_lt_dec rhs lhs); auto.
+    - apply le_lteq in l. apply le_lteq in l0.
+      des; auto. rewrite l in l0. apply lt_strorder in l0. done.
+    - rewrite l in l0. apply lt_strorder in l0. done.
+  Qed.
+
+  Lemma meet_assoc a b c: meet (meet a b) c = meet a (meet b c).
+  Proof.
+    unfold meet.
+    repeat
+      (try match goal with
+           | [H: le _ _ |- _] =>
+             apply le_lteq in H
+           | [|- context[le_lt_dec ?a ?b]] =>
+             destruct (le_lt_dec a b)
+           | [H: context[le_lt_dec ?a ?b] |- _] =>
+             destruct (le_lt_dec a b)
+           | [H1: lt ?a ?b, H2: lt ?b ?a |- _] =>
+             rewrite H2 in H1; apply lt_strorder in H1; inv H1
+           end; unfold eq in *; try subst; des; ss).
+    - rewrite l2 in l. rewrite l1 in l.
+      apply lt_strorder in l. inv l.
+    - rewrite l2 in l. rewrite l0 in l.
+      apply lt_strorder in l. inv l.
+  Qed.
+
+  Lemma meet_l lhs rhs:
+    le (meet lhs rhs) lhs.
+  Proof.
+    unfold meet. destruct (le_lt_dec lhs rhs); auto.
+    - apply le_lteq. auto.
+    - apply le_lteq. auto.
+  Qed.
+
+  Lemma meet_r lhs rhs:
+    le (meet lhs rhs) rhs.
+  Proof.
+    rewrite meet_comm. apply meet_l.
+  Qed.
+
+  Lemma meet_spec lhs rhs o
+        (LHS: le o lhs)
+        (RHS: le o rhs):
+    le o (meet lhs rhs).
+  Proof.
+    unfold meet. destruct (le_lt_dec lhs rhs); auto.
+  Qed.
+
+  Lemma meet_cases lhs rhs:
+    meet lhs rhs = lhs \/ meet lhs rhs = rhs.
+  Proof.
+    unfold meet. destruct (le_lt_dec lhs rhs); auto.
+  Qed.
+
+  Lemma eq_dec_eq A i (a1 a2:A):
+    (if eq_dec i i then a1 else a2) = a1.
+  Proof.
+    destruct (eq_dec i i); [|congruence]. auto.
+  Qed.
+
+  Lemma eq_dec_neq A i1 i2 (a1 a2:A)
+        (NEQ: i1 <> i2):
+    (if eq_dec i1 i2 then a1 else a2) = a2.
+  Proof.
+    destruct (eq_dec i1 i2); [congruence|]. auto.
+  Qed.
+
+  Lemma le_xI
+        lhs rhs
+        (LE: DOAux.le lhs rhs):
+    le (xI lhs) (xI rhs).
+  Proof.
+    inv LE.
+    - left. econs. auto.
+    - inv H. right. refl.
+  Qed.
+
+  Lemma le_xO
+        lhs rhs
+        (LE: DOAux.le lhs rhs):
+    le (xO lhs) (xO rhs).
+  Proof.
+    inv LE.
+    - left. econs. auto.
+    - inv H. right. refl.
+  Qed.
 End DenseOrder.
 
 Global Program Instance DenseOrder_le_PreOrder: PreOrder DenseOrder.le.
@@ -328,12 +633,13 @@ Next Obligation.
   left. rewrite H. auto.
 Qed.
 
+
 Module DOSet := UsualSet DenseOrder.
 
 Module DOMap.
   Include UsualPositiveMap.
 
-  Fixpoint raw_max_key A (m:Raw.t A): option DenseOrder.t :=
+  Fixpoint raw_max_key A (m:Raw.t A): option DOAux.t :=
     match m with
     | Raw.Leaf _ => None
     | Raw.Node l o r =>
@@ -360,13 +666,13 @@ Module DOMap.
   Lemma raw_max_key_spec2 A (m:Raw.t A) k
         (KEY: raw_max_key _ m = Some k):
     <<FIND: Raw.find k m <> None>> /\
-    <<MAX: forall k' (FIND': Raw.find k' m <> None), DenseOrder.le k' k>>.
+    <<MAX: forall k' (FIND': Raw.find k' m <> None), DOAux.le k' k>>.
   Proof.
     revert k KEY. induction m; s; [congr|].
     destruct (raw_max_key A m2) eqn:K2.
     { i. inv KEY. s. exploit IHm2; eauto. i. des.
       splits; eauto. i. destruct k'; ss.
-      - apply DenseOrder.le_xI. auto.
+      - apply DOAux.le_xI. auto.
       - left. econs.
       - left. econs.
     }
@@ -381,29 +687,67 @@ Module DOMap.
     { i. inv KEY. s. exploit IHm1; eauto. i. des.
       splits; eauto. i. destruct k'; ss.
       - erewrite raw_max_key_spec1 in FIND'; eauto. congr.
-      - apply DenseOrder.le_xO. auto.
+      - apply DOAux.le_xO. auto.
       - congr.
     }
     i. congr.
   Qed.
 
   Definition max_key A (m:t A): DenseOrder.t :=
-    match raw_max_key A (proj1_sig m)  with
-    | Some k => k
-    | None => DenseOrder.elt
+    match proj1_sig m with
+    | Raw.Leaf _ => DenseOrder.bot
+    | Raw.Node l o r =>
+      match raw_max_key _ r, raw_max_key _ l, o with
+      | Some k, _, _ => xI k
+      | None, Some k, _ => xO k
+      | None, None, Some _ => xH
+      | None, None, None => DenseOrder.bot
+      end
     end.
 
   Lemma max_key_spec A (m:t A):
-    <<FIND: find DenseOrder.elt m <> None -> find (max_key _ m) m <> None>> /\
+    <<FIND: forall k', find k' m <> None -> find (max_key _ m) m <> None>> /\
     <<MAX: forall k' (FIND': find k' m <> None), DenseOrder.le k' (max_key _ m)>>.
   Proof.
-    unfold max_key. destruct (raw_max_key A (proj1_sig m)) eqn:X.
-    - exploit raw_max_key_spec2; eauto. i. des. splits; i.
-      + unfold find. auto.
-      + apply MAX. auto.
-    - splits; i.
-      + unfold find in H. erewrite raw_max_key_spec1 in H; eauto.
-      + unfold find in FIND'. erewrite raw_max_key_spec1 in FIND'; eauto. congr.
+    destruct m.
+    unfold max_key, find. s. destruct x eqn:X; subst.
+    { splits; i.
+      + rewrite PositiveMap.gleaf in H. congr.
+      + rewrite PositiveMap.gleaf in FIND'. congr.
+    }
+    destruct (raw_max_key A t0_2) eqn:Y.
+    { exploit raw_max_key_spec2; eauto. i. des. splits; i; auto.
+      destruct k'; ss.
+      - exploit MAX; eauto. i. inv x.
+        + left. econs. eauto.
+        + right. inv H. refl.
+      - left. econs.
+      - left. econs.
+    }
+    destruct (raw_max_key A t0_1) eqn:Z.
+    { exploit raw_max_key_spec2; eauto. i. des. splits; i; auto.
+      destruct k'; ss.
+      - erewrite raw_max_key_spec1 in FIND'; eauto. congr.
+      - exploit MAX; eauto. i. inv x.
+        + left. econs. eauto.
+        + right. inv H. refl.
+      - left. econs.
+    }
+    destruct o.
+    { s. i. splits; i; [congr|].
+      destruct k'; ss.
+      - erewrite raw_max_key_spec1 in FIND'; eauto. congr.
+      - erewrite raw_max_key_spec1 in FIND'; eauto. congr.
+      - refl.
+    }
+    s. splits; i.
+    - destruct k'; ss.
+      + erewrite raw_max_key_spec1 in H; eauto.
+      + erewrite raw_max_key_spec1 in H; eauto.
+    - destruct k'; ss.
+      + erewrite raw_max_key_spec1 in FIND'; eauto. congr.
+      + erewrite raw_max_key_spec1 in FIND'; eauto. congr.
+      + refl.
   Qed.
 End DOMap.
 
